Utils/Tactics.v
@@ -5,9 +5,9 @@ From Warblre Require Import Base.
 (* Tactic for rewriting decidable equalities into propositional ones *)
 Ltac eqdec := repeat match goal with
   | [ H: (?x ==? ?y)%wt = true |- _ ] => rewrite EqDec.inversion_true in H; subst
-  | [ H: (?x ==? ?y)%wt = false |- _ ] => rewrite EqDec.inversion_false in H
-  | [ |- (?x ==? ?y)%wt = true ] => rewrite EqDec.inversion_true
-  | [ |- (?x ==? ?y)%wt = false ] => rewrite EqDec.inversion_false
+  | [ H: context[(?x ==? ?y)%wt = false] |- _ ] => rewrite EqDec.inversion_false in H
+  | [ |- context[(?x ==? ?y)%wt = true] ] => rewrite EqDec.inversion_true
+  | [ |- context[(?x ==? ?y)%wt = false] ] => rewrite EqDec.inversion_false
   | [ |- context[(?x ==? ?y)%wt] ] => destruct (x ==? y)%wt eqn:?Heq
   | [ H: context[(?x ==? ?y)%wt] |- _ ] => destruct (x ==? y)%wt eqn:?Heq
 end.
